expand set definitions

Valaig/ForLean/Set.lean
@@ -7,15 +7,169 @@ variable {α : Type u}
 /--
   Basic set definition as a predicate on a type.
 -/
-def Set (α : Type u) := α -> Prop
+def Set (α : Type u) :=
+  α -> Prop
 
 namespace Set
+variable {s : Set α} {a : α}
+
+def ofFn (f : α -> Prop) : Set α :=
+  f
 
 instance : Membership α (Set α) where
   mem s a := s a
 
-theorem mem_iff {s : Set α} {a : α} :
+@[local grind =]
+theorem mem_iff :
     a ∈ s ↔ s a := by
   rfl
+
+@[simp, grind =]
+theorem mem_ofFn {f : α -> Prop} :
+    a ∈ ofFn f ↔ f a := by
+  rfl
+
+@[ext, grind ext]
+theorem ext_mem {a b : Set α} (h : ∀ x, x ∈ a ↔ x ∈ b) :
+    a = b := by
+  funext x
+  simp [←mem_iff, h]
+
+def compl (set : Set α) : Set α :=
+  (· ∉ set)
+
+@[simp, grind =]
+theorem mem_compl :
+    a ∈ s.compl ↔ a ∉ s := by
+  grind [compl]
+
+def filter (set : Set α) (p : α -> Prop) : Set α :=
+  fun x => x ∈ set ∧ p x
+
+@[simp, grind =]
+theorem mem_filter {p : α -> Prop} :
+    a ∈ s.filter p ↔ a ∈ s ∧ p a := by
+  grind [filter]
+
+def empty : Set α :=
+  fun _ => False
+
+@[simp, grind .]
+theorem mem_empty :
+    a ∉ empty := by
+  grind [empty]
+
+instance : Inhabited (Set α) where
+  default := empty
+
+def bottom : Set α :=
+  empty
+
+@[simp, grind =]
+theorem bottom_eq :
+    (bottom : Set α) = empty := by
+  rfl
+
+def top : Set α :=
+  bottom.compl
+
+@[simp, grind .]
+theorem mem_top :
+    a ∈ top := by
+  simp [top]
+
+instance : EmptyCollection (Set α) where
+  emptyCollection := bottom
+
+@[simp]
+theorem emptyCollection_eq :
+    (EmptyCollection.emptyCollection : Set α) = bottom := by
+  rfl
+
+instance : Insert α (Set α) where
+  insert a s := fun x => x ∈ s ∨ x = a
+
+@[simp, grind =]
+theorem mem_insert {x : α} :
+    a ∈ insert x s ↔ a ∈ s ∨ a = x := by
+  rfl
+
+instance : Singleton α (Set α) where
+  singleton a := (· = a)
+
+@[simp, grind =]
+theorem mem_singleton {x : α} :
+    a ∈ (singleton x : Set α) ↔ a = x := by
+  rfl
+
+instance : LawfulSingleton α (Set α) where
+  insert_empty_eq := by simp; grind
+
+instance : HasSubset (Set α) where
+  Subset a b := ∀ x ∈ a, x ∈ b
+
+instance : HasSSubset (Set α) where
+  SSubset a b := a ⊆ b ∧ ∃ x ∈ b, x ∉ a
+
+instance : Union (Set α) where
+  union a b := fun x => x ∈ a ∨ x ∈ b
+
+@[simp, grind =]
+theorem mem_union {a b : Set α} {x : α} :
+    x ∈ a ∪ b ↔ x ∈ a ∨ x ∈ b := by
+  rfl
+
+instance : Inter (Set α) where
+  inter a b := fun x => x ∈ a ∧ x ∈ b
+
+@[simp, grind =]
+theorem mem_inter {a b : Set α} {x : α} :
+    x ∈ a ∩ b ↔ x ∈ a ∧ x ∈ b := by
+  rfl
+
+instance : SDiff (Set α) where
+  sdiff a b := fun x => x ∈ a ∧ x ∉ b
+
+@[simp, grind =]
+theorem mem_sdiff {a b : Set α} {x : α} :
+    x ∈ a \ b ↔ x ∈ a ∧ x ∉ b := by
+  rfl
+
+instance : Pure Set where
+  pure a := singleton a
+
+@[simp, grind =]
+theorem mem_pure {x : α} :
+    (pure x : Set α) = singleton x := by
+  rfl
+
+instance : Bind Set where
+  bind s f := fun b => ∃ a ∈ s, b ∈ f a
+
+@[simp, grind =]
+theorem mem_bind {β : Type u} {x : β} {f : α -> Set β} :
+    x ∈ (s >>= f) ↔ ∃ a ∈ s, x ∈ f a := by
+  rfl
+
+def map {β : Type v} (s : Set α) (f : α -> β) : Set β :=
+  fun b => ∃ a ∈ s, b = f a
+
+@[simp, grind =]
+theorem mem_map {β : Type v} {x : β} {f : α -> β} :
+    x ∈ s.map f ↔ ∃ a ∈ s, x = f a := by
+  rfl
+
+instance : Functor Set where
+  map f s := s.map f
+
+@[simp, grind =]
+theorem functor_map_eq {β : Type u} {f : α -> β} :
+    map s f = s.map f := by
+  rfl
+
+instance : LawfulFunctor Set where
+  map_const := by simp +instances [instFunctor]
+  id_map := by simp +instances only [instFunctor]; grind
+  comp_map := by simp +instances only [instFunctor]; grind
 
 end Valaig.Set
